src/cddl/spec/CDDL.Spec.Map.fsti
@@ -4,72 +4,69 @@ module U = CBOR.Spec.Util
 module S = CDDL.Spec.Set
 
 val t
-  (#key: Type)
-  (#key_s: typ)
-  (spec_key: spec key_s key true)
+  (key: Type0)
   ([@@@strictly_positive] value: Type u#a)
 : Tot (Type u#a)
 
 val get
   (#key: Type)
-  (#key_s: typ)
-  (#spec_key: spec key_s key true)
   (#value: Type)
-: t spec_key value -> key -> Tot (option value)
+: t key value -> key -> Tot (option value)
 
 let defined
   (#key: Type)
-  (#key_s: typ)
-  (#spec_key: spec key_s key true)
   (#value: Type)
-  (k: key) (f: t spec_key value)
+  (k: key) (f: t key value)
 : Tot bool
 = Some? (get f k)
 
 let equal
   (#key: Type)
-  (#key_s: typ)
-  (#spec_key: spec key_s key true)
   (#value: Type)
-  (m1 m2: t spec_key value)
+  (m1 m2: t key value)
 : Tot prop =
   (forall k . get m1 k == get m2 k)
 
 val ext
   (#key: Type)
-  (#key_s: typ)
-  (#spec_key: spec key_s key true)
   (#value: Type)
-  (m1 m2: t spec_key value)
+  (m1 m2: t key value)
 : Lemma
   (ensures (equal m1 m2 <==> m1 == m2))
   [SMTPat (equal m1 m2)]
 
 let mem
   (#key: Type)
-  (#key_s: typ)
-  (#spec_key: spec key_s key true)
   (#value: Type)
   (kv: (key & value))
-  (f: t spec_key value)
+  (f: t key value)
 : Tot prop
 = get f (fst kv) == Some (snd kv)
 
+let mem_defined
+  (#key: Type)
+  (#value: Type)
+  (k: key)
+  (f: t key value)
+: Lemma
+  (match get f k with
+  | None -> True
+  | Some v -> mem (k, v) f
+  )
+  [SMTPat (get f k)]
+= ()
+
 let equal'
   (#key: Type)
-  (#key_s: typ)
-  (#spec_key: spec key_s key true)
   (#value: Type)
-  (m1 m2: t spec_key value)
+  (m1 m2: t key value)
 : Tot prop =
   (forall kv . mem kv m1 <==> mem kv m2)
 
 let ext'
   (#key: Type)
-  (#key_s: typ)
-  (#spec_key: spec key_s key true)
   (#value: Type)
-  (m1 m2: t spec_key value)
+  (m1 m2: t key value)
 : Lemma
   (ensures (equal' m1 m2 <==> m1 == m2))
   [SMTPat (equal' m1 m2)]
@@ -91,114 +88,87 @@ let ext'
 
 val length
   (#key: Type)
-  (#key_s: typ)
-  (#spec_key: spec key_s key true)
   (#value: Type)
-  (m: t spec_key value)
+  (m: t key value)
 : Tot nat
 
 val key_set
   (#key: Type)
   (#key_s: typ)
-  (#spec_key: spec key_s key true)
+  (spec_key: spec key_s key true)
   (#value: Type)
-  (m: t spec_key value)
+  (m: t key value)
 : Pure (S.t spec_key)
-    (requires True)
+    (requires (
+      forall (x: key) . defined x m ==> spec_key.serializable x
+    ))
     (ensures fun s ->
       S.cardinality s == length m /\
       (forall x . S.mem x s <==> defined x m)
     )
 
-let defined_serializable
-  (#key: Type)
-  (#key_s: typ)
-  (#spec_key: spec key_s key true)
-  (#value: Type)
-  (m: t spec_key value)
-  (k: key)
-: Lemma
-  (ensures (defined k m ==> spec_key.serializable k))
-  [SMTPat (get m k)]
-= assert (defined k m ==> S.mem k (key_set m))
-
 val empty
-  (#key: Type)
-  (#key_s: typ)
-  (spec_key: spec key_s key true)
+  (key: Type)
   (value: Type u#a)
-: t spec_key value
+: t key value
 
 val get_empty
   (#key: Type)
-  (#key_s: typ)
-  (spec_key: spec key_s key true)
   (value: Type u#a)
   (k: key)
 : Lemma
-  (ensures (get (empty spec_key value) k == None))
-  [SMTPat (get (empty spec_key value) k)]
+  (ensures (get (empty key value) k == None))
+  [SMTPat (get (empty key value) k)]
 
-let length_empty
-  (#key: Type)
-  (#key_s: typ)
-  (spec_key: spec key_s key true)
+val length_empty
+  (key: Type)
   (value: Type u#a)
 : Lemma
-  (ensures (length (empty spec_key value) == 0))
-  [SMTPat (length (empty spec_key value))]
-= assert (S.equal (key_set (empty spec_key value)) (S.emptyset spec_key))
+  (ensures (length (empty key value) == 0))
+  [SMTPat (length (empty key value))]
 
 val singleton
   (#key: Type)
-  (#key_s: typ)
-  (spec_key: spec key_s key true)
   (#value: Type u#a)
-  (k: key { spec_key.serializable k })
+  (k: key)
+  (k_eq: ((k' : key) -> Pure bool True (fun res -> res == true <==> k'  == k)))
   (v: value)
-: t spec_key value
+: t key value
 
 val get_singleton
   (#key: Type)
-  (#key_s: typ)
-  (spec_key: spec key_s key true)
   (#value: Type u#a)
-  (k: key { spec_key.serializable k })
+  (k: key)
+  (k_eq: ((k' : key) -> Pure bool True (fun res -> res == true <==> k'  == k)))
   (v: value)
   (k': key)
 : Lemma
   (ensures (
-    let v' = get (singleton spec_key k v) k' in
+    let v' = get (singleton k k_eq v) k' in
     (k == k' ==> v' == Some v) /\
     ((~ (k == k')) ==> v' == None)
   ))
-  [SMTPat (get (singleton spec_key k v) k')]
+  [SMTPat (get (singleton k k_eq v) k')]
 
-let length_singleton
+val length_singleton
   (#key: Type)
-  (#key_s: typ)
-  (spec_key: spec key_s key true)
   (#value: Type u#a)
-  (k: key { spec_key.serializable k })
+  (k: key)
+  (k_eq: ((k' : key) -> Pure bool True (fun res -> res == true <==> k'  == k)))
   (v: value)
 : Lemma
-  (ensures (length (singleton spec_key k v) == 1))
-  [SMTPat (length (singleton spec_key k v))]
-= assert (S.equal (key_set (singleton spec_key k v)) (S.singleton spec_key k))
+  (ensures (length (singleton k k_eq v) == 1))
+  [SMTPat (length (singleton k k_eq v))]
 
 val union
   (#key: Type)
-  (#key_s: typ)
-  (#spec_key: spec key_s key true)
   (#value: Type u#a)
-: t spec_key value -> t spec_key value -> t spec_key value
+: t key value -> t key value -> t key value
 
 val get_union
   (#key: Type)
-  (#key_s: typ)
-  (#spec_key: spec key_s key true)
   (#value: Type u#a)
-: (m1: t spec_key value) -> (m2: t spec_key value) -> (k: key) -> Lemma
+: (m1: t key value) -> (m2: t key value) -> (k: key) -> Lemma
   (ensures (get (union m1 m2) k == begin match get m1 k with
     | None -> get m2 k
     | v -> v
@@ -208,33 +178,25 @@ val get_union
 
 let disjoint
   (#key: Type)
-  (#key_s: typ)
-  (#spec_key: spec key_s key true)
   (#value: Type u#a)
-  (m1 m2: t spec_key value)
+  (m1 m2: t key value)
 : Tot prop =
   forall k . ~ (defined k m1 /\ defined k m2)
 
-let length_disjoint_union
+val length_disjoint_union
   (#key: Type)
-  (#key_s: typ)
-  (#spec_key: spec key_s key true)
   (#value: Type u#a)
-  (m1 m2: t spec_key value)
+  (m1 m2: t key value)
 : Lemma
   (requires (disjoint m1 m2))
   (ensures (
     length (union m1 m2) == length m1 + length m2
   ))
-= assert (S.equal (key_set (union m1 m2)) (S.union (key_set m1) (key_set m2)));
-  S.disjoint_union_cardinality (key_set m1) (key_set m2)
 
 let union_assoc
   (#key: Type)
-  (#key_s: typ)
-  (#spec_key: spec key_s key true)
   (#value: Type u#a)
-  (m1 m2 m3: t spec_key value)
+  (m1 m2 m3: t key value)
 : Lemma
   (union (union m1 m2) m3 == union m1 (union m2 m3))
 = ext
@@ -243,10 +205,8 @@ let union_assoc
 
 let union_empty_l
   (#key: Type)
-  (#key_s: typ)
-  (#spec_key: spec key_s key true)
   (#value: Type u#a)
-  (m: t spec_key value)
+  (m: t key value)
 : Lemma
   (union (empty _ _) m == m)
   [SMTPat (union (empty _ _) m)]
@@ -254,10 +214,8 @@ let union_empty_l
 
 let union_empty_r
   (#key: Type)
-  (#key_s: typ)
-  (#spec_key: spec key_s key true)
   (#value: Type u#a)
-  (m: t spec_key value)
+  (m: t key value)
 : Lemma
   (union m (empty _ _) == m)
   [SMTPat (union m (empty _ _))]
@@ -265,10 +223,8 @@ let union_empty_r
 
 let disjoint_union_comm
   (#key: Type)
-  (#key_s: typ)
-  (#spec_key: spec key_s key true)
   (#value: Type u#a)
-  (m1 m2: t spec_key value)
+  (m1 m2: t key value)
 : Lemma
   (requires disjoint m1 m2)
   (ensures m1 `union` m2 == m2 `union` m1)
@@ -277,20 +233,16 @@ let disjoint_union_comm
 
 val filter
   (#key: Type)
-  (#key_s: typ)
-  (#spec_key: spec key_s key true)
   (#value: Type u#a)
 :
   ((key & value) -> bool) ->
-  t spec_key value ->
-  t spec_key value
+  t key value ->
+  t key value
 
 val get_filter
   (#key: Type)
-  (#key_s: typ)
-  (#spec_key: spec key_s key true)
   (#value: Type u#a)
-: (f: (key & value -> bool)) -> (m: t spec_key value) -> (k: key) -> Lemma
+: (f: (key & value -> bool)) -> (m: t key value) -> (k: key) -> Lemma
   (ensures (get (filter f m) k == begin match get m k with
   | None -> None
   | Some v -> if f (k, v) then Some v else None
@@ -299,11 +251,9 @@ val get_filter
 
 let filter_ext
   (#key: Type)
-  (#key_s: typ)
-  (#spec_key: spec key_s key true)
   (#value: Type u#a)
   (f1 f2: (key & value) -> Tot bool)
-  (m: t spec_key value)
+  (m: t key value)
 : Lemma
   (requires forall x . f1 x == f2 x)
   (ensures filter f1 m == filter f2 m)
@@ -311,11 +261,9 @@ let filter_ext
 
 let disjoint_union_filter
   (#key: Type)
-  (#key_s: typ)
-  (#spec_key: spec key_s key true)
   (#value: Type u#a)
   (f: (key & value) -> Tot bool)
-  (m1 m2: t spec_key value)
+  (m1 m2: t key value)
 : Lemma
   (requires disjoint m1 m2)
   (ensures (filter f (union m1 m2) == filter f m1 `union` filter f m2))
@@ -325,11 +273,9 @@ let disjoint_union_filter
 
 let filter_filter
   (#key: Type)
-  (#key_s: typ)
-  (#spec_key: spec key_s key true)
   (#value: Type u#a)
   (p1 p2: (key & value) -> Tot bool)
-  (f: t spec_key value)
+  (f: t key value)
 : Lemma
   (filter p2 (filter p1 f) == filter (p1 `U.andp` p2) f)
 = ext
@@ -338,27 +284,30 @@ let filter_filter
 
 let filter_implies
   (#key: Type)
-  (#key_s: typ)
-  (#spec_key: spec key_s key true)
   (#value: Type u#a)
   (p1 p2: (key & value) -> Tot bool)
-  (f: t spec_key value)
+  (f: t key value)
 : Lemma
   (requires (forall kv . p1 kv ==> p2 kv))
   (ensures (filter p2 (filter p1 f) == filter p1 f))
 = filter_filter p1 p2 f;
   filter_ext p1 (p1 `U.andp` p2) f
 
-let for_all
+val for_all
   (#key: Type)
-  (#key_s: typ)
-  (#spec_key: spec key_s key true)
   (#value: Type u#a)
   (f: (key & value -> bool))
-  (m: t spec_key value)
+  (m: t key value)
 : Pure bool
     (requires True)
     (ensures fun b -> b <==> (forall kv . mem kv m ==> f kv))
-= let b = (key_set (filter f m) = key_set m) in // HERE we use the fact that the key set is eqtype
-  assert (b == true <==> equal (filter f m) m);
-  b
+
+let for_all_keys
+  (#key: Type)
+  (#value: Type u#a)
+  (f: (key -> bool))
+  (m: t key value)
+: Pure bool
+    (requires True)
+    (ensures fun b -> b <==> (forall k . defined k m ==> f k))
+= for_all (fun kv -> f (fst kv)) m
